WIP

src/tls/Handshake.fst
@@ -55,7 +55,7 @@ let prepareClientHello cfg ks log ri sido =
    ch_cipher_suites = co.co_cipher_suites;
    ch_raw_cipher_suites = None;
    ch_compressions = co.co_compressions;
-   ch_extensions = Some ext;} in
+   ch_extensions = ext;} in
   let chb = log @@ (ClientHello ch) in
   (ClientHello ch, chb)
 
@@ -91,45 +91,52 @@ let getCachedSession cfg cg = None
 #set-options "--lax"
 
 // FIXME: TLS1.3
-val prepareServerHello: config -> KeySchedule.ks -> HandshakeLog.log -> option ri -> (hs_msg * bytes) -> ST (result (nego * option KeySchedule.recordInstance * (hs_msg * bytes)))
+val prepareServerHello: config -> KeySchedule.ks -> HandshakeLog.log -> option ri -> (hs_msg * bytes) -> ST (result (sessionInfo * option KeySchedule.recordInstance * (hs_msg * bytes)))
   (requires (fun h -> True))
   (ensures (fun h0 i h1 -> True))
 let prepareServerHello cfg ks log ri (ClientHello ch,_) =
- let mode = computeMode cfg ch.ch_protocol_version ch.ch_cipher_suites ch.ch_extensions ch.ch_compressions ri in  
+ let mode, sext, sext_ee = computeMode cfg ch.ch_protocol_version ch.ch_cipher_suites ch.ch_extensions ch.ch_compressions ri in  
   match mode with
    | Error(z) -> Error(z)
    | Correct(mode) ->
   let srand = KeySchedule.ks_server_random ks in
-  let ksl = 
+  let sext = 
     (match mode.m_protocol_version, mode.m_dh_group, mode.m_dh_share with
      | TLS_1p3, Some gn, Some gxb -> 
        let gyb = KeySchedule.ks_server_13_1rtt_init ks ch.ch_client_random mode.m_cipher_suite gn gxb in
-       (Some (ServerKeyShare (gn,gyb)))
-     | _ -> None) in
-  let sext = negotiateServerExtensions mode.m_protocol_version ch.ch_extensions ch.ch_cipher_suites cfg mode.m_cipher_suite ri ksl false in
+       (ServerKeyShare (gn,gyb)) :: sext
+     | _ -> sext) in
   let sid = CoreCrypto.random 32 in
   let sh = 
    {sh_protocol_version = mode.m_protocol_version;
-    sh_sessionID = Some sid;
+    sh_sessionID = sid;
     sh_server_random = srand;
     sh_cipher_suite = mode.m_cipher_suite;
     sh_compression = mode.m_comp;
     sh_extensions = sext} in
-  let nego = 
-   {n_client_random = ch.ch_client_random;
-    n_server_random = srand;
-    n_sessionID = Some sid;
-    n_protocol_version = mode.m_protocol_version;
-    n_kexAlg = mode.m_kexAlg;
-    n_sigAlg = mode.m_sigAlg;
-    n_aeAlg  = mode.m_aeAlg;
-    n_cipher_suite = mode.m_cipher_suite;
-    n_compression = mode.m_comp;
-    n_dh_group = mode.m_dh_group;
-    n_scsv = [];
-    n_extensions = mode.m_ext;
-    (* [getCachedSession] returned [None], so no session resumption *)
-    n_resume = false} in
+  let si = {
+    si_resume = false;
+    si_client_random = ch.ch_client_random;
+    si_server_random = srand;
+    si_protocol_version = mode.m_protocol_version;
+    si_sessionID = sid;
+    si_sessiosi_hash = None:
+    si_kexAlg = mode.m_kexAlg;
+    si_aeAlg = mode.m_aeAlg;
+    si_server_cert = mode.m_server_cert;
+    si_sigAlg = mode.m_sigAlg;
+    si_cipher_suite = mode.m_cipher_suite;
+    si_dh_group = mode.m_dh_group;
+    si_compression = mode.m_comp:
+    si_extended_ms = mode.m_extended_ms;
+    si_extended_padding = mode.m_extended_padding;
+    si_secure_renegotiation = m_secure_renegotiation;
+    si_point_format = mode.m_point_format;
+    si_server_name = mode.m_server_name;
+    si_client_auth = false;
+    si_clientID = None;
+    si_clientSigAlg = None;
+  } in
   let _ = log @@ (ClientHello ch) in
   let shb = log @@ (ServerHello sh) in
   let keys = (match mode.m_protocol_version with
@@ -137,11 +144,11 @@ let prepareServerHello cfg ks log ri (ClientHello ch,_) =
 	       let keys = KeySchedule.ks_server_13_sh ks in
 	       Some keys
 	     | _ -> None) in
-    Correct (nego,keys,(ServerHello sh,shb))
+    Correct (si, keys, (ServerHello sh,shb))
 
   
 val processServerHello: c:config -> KeySchedule.ks -> HandshakeLog.log -> option ri -> ch -> (hs_msg * bytes) ->
-  ST (result (nego * option KeySchedule.recordInstance))
+  ST (result (sessionInfo * option KeySchedule.recordInstance))
      (requires (fun h -> True))
      (ensures (fun h0 i h1 -> True))
 let processServerHello cfg ks log ri ch (ServerHello sh,_) =
@@ -149,21 +156,30 @@ let processServerHello cfg ks log ri ch (ServerHello sh,_) =
   let mode = computeClientMode cfg ch.ch_extensions ch.ch_protocol_version sh.sh_protocol_version sh.sh_server_random sh.sh_cipher_suite sh.sh_extensions sh.sh_compression ri in
    match mode with
     | Error(z) -> Error(z)
-    | Correct(mode) ->  
-   let o_nego = 
-    {n_client_random = ch.ch_client_random;
-     n_server_random = sh.sh_server_random;
-     n_sessionID = sh.sh_sessionID;
-     n_protocol_version = mode.m_protocol_version;
-     n_kexAlg = mode.m_kexAlg;
-     n_aeAlg = mode.m_aeAlg;
-     n_sigAlg = mode.m_sigAlg;
-     n_cipher_suite = mode.m_cipher_suite;
-     n_dh_group = mode.m_dh_group;
-     n_compression = sh.sh_compression;
-     n_scsv = [];
-     n_extensions = mode.m_ext;
-     n_resume = false } in
+    | Correct(mode) -> 
+    let si = {
+      si_resume = false;
+      si_client_random = ch.ch_client_random;
+      si_server_random = sh.sh_server_random;
+      si_protocol_version = mode.m_protocol_version;
+      si_sessionID = sh.sh_sessionID;
+      si_sessiosi_hash = None:
+      si_kexAlg = mode.m_kexAlg;
+      si_aeAlg = mode.m_aeAlg;
+      si_server_cert = mode.m_server_cert;
+      si_sigAlg = mode.m_sigAlg;
+      si_cipher_suite = mode.m_cipher_suite;
+      si_dh_group = mode.m_dh_group;
+      si_compression = mode.m_comp:
+      si_extended_ms = mode.m_extended_ms;
+      si_extended_padding = mode.m_extended_padding;
+      si_secure_renegotiation = m_secure_renegotiation;
+      si_point_format = mode.m_point_format;
+      si_server_name = mode.m_server_name;
+      si_client_auth = false;
+      si_clientID = None;
+      si_clientSigAlg = None;
+    } in
     (match o_nego.n_protocol_version, o_nego.n_kexAlg, mode.m_dh_group, mode.m_dh_share with
      | TLS_1p3, Kex_DHE, Some gn, Some gyb 
      | TLS_1p3, Kex_ECDHE, Some gn, Some gyb -> 
