src/tls/TLSInfo.fst
@@ -95,8 +95,8 @@ noeq type config = {
 
     (* Server side *)
     request_client_certificate: bool; // TODO: generalize to CertificateRequest contents: a list of CAs.
-    check_client_version_in_pms_for_old_tls: bool;
-    cert_chain_file: string;    // TEMPORARY until the proper cert logic described above is implemented
+    check_client_versiosi_isi_pms_for_old_tls: bool;
+    cert_chaisi_file: string;    // TEMPORARY until the proper cert logic described above is implemented
     private_key_file: string;   // TEMPORARY
 
     (* Common *)
@@ -164,8 +164,8 @@ let defaultConfig =
     allowAnonCipherSuite = false;
 
     request_client_certificate = false;
-    check_client_version_in_pms_for_old_tls = true;
-    cert_chain_file = "server.pem";
+    check_client_versiosi_isi_pms_for_old_tls = true;
+    cert_chaisi_file = "server.pem";
     private_key_file = "server.key";
 
     safe_renegotiation = true;
@@ -218,7 +218,7 @@ type ri_status =
 
 // Placeholder for overhaul of 1.2 indexes
 type pmsId = PMS.pms
-assume val strongKEX: pmsId -> Tot bool
+assume val strongKEX: kexAlg -> Tot bool
 
 // -------------------------------------------------------------------
 // Master Secret indexes and their properties
@@ -239,37 +239,34 @@ type sessionID = b:bytes { length b <= 32 }
 // ``An arbitrary byte sequence chosen by the server
 // to identify an active or resumable session state.''
 
-noeq type nego = {
-  n_resume: bool;
-  n_client_random: random;
-  n_server_random: random;
-  n_protocol_version: protocolVersion;
-  n_sessionID: option sessionID;
-  n_session_hash: sessionHash;
-  n_kexAlg: kexAlg;
-  n_aeAlg: aeAlg;
-  n_server_cert: option Cert.chain;
-  n_sigAlg: option sigAlg;
-  n_cipher_suite: cipherSuite;
-  n_dh_group: option namedGroup;
-  n_compression: option compression;
-  n_extended_ms: bool;
-  n_extended_padding: bool;
-  n_secure_renegotiation: ri_status;
-  n_point_format: option ECGroup.point_format;
-  n_server_name: option serverName;
-  n_client_auth: bool;
-  n_clientID: option Cert.chain;
-  n_clientSigAlg: option sigHashAlg;
-  n_pmsId: PMS.pms;
+noeq type sessionInfo = {
+  si_resume: bool;
+  si_client_random: random;
+  si_server_random: random;
+  si_protocol_version: protocolVersion;
+  si_sessionID: sessionID;
+  si_sessiosi_hash: sessionHash;
+  si_kexAlg: kexAlg;
+  si_aeAlg: aeAlg;
+  si_server_cert: option Cert.chain;
+  si_sigAlg: option sigAlg;
+  si_cipher_suite: cipherSuite;
+  si_dh_group: option namedGroup;
+  si_compression: option compression;
+  si_extended_ms: bool;
+  si_extended_padding: bool;
+  si_secure_renegotiation: ri_status;
+  si_point_format: option ECGroup.point_format;
+  si_server_name: option serverName;
+  si_client_auth: bool;
+  si_clientID: option Cert.chain;
+  si_clientSigAlg: option sigHashAlg;
 }
-
-type session_info = nego
 
 type abbrInfo =
     {abbr_crand: crand;
      abbr_srand: srand;
-     abbr_session_hash: sessionHash;
+     abbr_sessiosi_hash: sessionHash;
      abbr_vd: option (cVerifyData * sVerifyData) }
 
 // for sessionID. we treat empty bytes as the absence of identifier,
@@ -278,8 +275,8 @@ type abbrInfo =
 // for certificates, the empty list represents the absence of identity
 // (possibly refusing to present requested certs)
 
-val csrands: session_info -> Tot csRands
-let csrands si = si.n_client_random @| si.n_server_random
+val csrands: sessionInfo -> Tot csRands
+let csrands si = si.si_client_random @| si.si_server_random
 //CF subsumes mk_csrands
 
 // Getting algorithms from nego
@@ -301,11 +298,11 @@ let kdfAlg pv cs =
   | TLS_1p2           -> PRF_TLS_1p2 kdf_label (prfMacAlg_of_ciphersuite cs)
   | TLS_1p3           -> PRF_TLS_1p3 //TBC
 
-let vdAlg si = si.n_protocol_version, si.n_cipher_suite
+let vdAlg si = si.si_protocol_version, si.si_cipher_suite
 
-val siAuthEncAlg: si:nego { si.n_protocol_version = TLS_1p2 &&
-                              pvcs si.n_protocol_version si.n_cipher_suite } -> Tot aeAlg
-let siAuthEncAlg si = get_aeAlg si.n_cipher_suite
+val siAuthEncAlg: si:sessionInfo { si.si_protocol_version = TLS_1p2 &&
+                              pvcs si.si_protocol_version si.si_cipher_suite } -> Tot aeAlg
+let siAuthEncAlg si = get_aeAlg si.si_cipher_suite
 
 type msId = // We record the parameters used to derive the master secret;
   | StandardMS : pmsId -> csRands -> kefAlg_t -> msId
@@ -333,13 +330,15 @@ let honestMS = function
 
 // Getting master-secret indexes out of nego
 
+(*
 //CF subsumes both MsI and mk_msid
-val msid: si:session_info { is_Some (prfMacAlg_of_ciphersuite_aux (si.n_cipher_suite)) } -> Tot msId
+val msid: si:sessionInfo { is_Some (prfMacAlg_of_ciphersuite_aux (si.si_cipher_suite)) } -> Tot msId
 let msid si =
-  let ems = si.n_extended_ms in
-  let kef = kefAlg si.n_protocol_version si.n_cipher_suite ems in
-  if ems then ExtendedMS si.n_pmsId si.n_session_hash kef
-  else StandardMS si.n_pmsId    (csrands si) kef
+  let ems = si.si_extended_ms in
+  let kef = kefAlg si.si_protocol_version si.si_cipher_suite ems in
+  if ems then ExtendedMS si.si_pmsId si.si_sessiosi_hash kef
+  else StandardMS si.si_pmsId    (csrands si) kef
+*)
 
 // Strengths of Handshake algorithms
 
@@ -354,17 +353,17 @@ assume val sigHashAlg_of_ciphersuite: cipherSuite -> Tot sigHashAlg
 
 // ``The algorithms of si are strong for both KDF and VerifyData, despite all others'
 // guarding idealization in PRF
-val strongPRF: si:nego{si.n_protocol_version = TLS_1p2 ==> ~(is_NullCipherSuite si.n_cipher_suite \/ is_SCSV si.n_cipher_suite) /\ is_Some (prfMacAlg_of_ciphersuite_aux si.n_cipher_suite)} -> Tot bool
-let strongPRF si = strongKDF(kdfAlg si.n_protocol_version si.n_cipher_suite) && strongVD(vdAlg si)
+val strongPRF: si:sessionInfo{si.si_protocol_version = TLS_1p2 ==> ~(is_NullCipherSuite si.si_cipher_suite \/ is_SCSV si.si_cipher_suite) /\ is_Some (prfMacAlg_of_ciphersuite_aux si.si_cipher_suite)} -> Tot bool
+let strongPRF si = strongKDF(kdfAlg si.si_protocol_version si.si_cipher_suite) && strongVD(vdAlg si)
 // MK I think having this joint strength predicate
 // MK guaranteeing the idealization of the complete module is useful
 
 // Summarizing all assumptions needed for a strong handshake
 // CF derived & to be used in the public API only
 let strongHS si =
-  strongKEX (si.n_pmsId) &&
-  is_Some (prfMacAlg_of_ciphersuite_aux si.n_cipher_suite) && //NS: needed to add this ...
-  strongKEF (kefAlg si.n_protocol_version si.n_cipher_suite si.n_extended_ms) && //NS: ... to verify this
+  strongKEX (si.si_kexAlg) &&
+  is_Some (prfMacAlg_of_ciphersuite_aux si.si_cipher_suite) && //NS: needed to add this ...
+  strongKEF (kefAlg si.si_protocol_version si.si_cipher_suite si.si_extended_ms) && //NS: ... to verify this
   strongPRF si
   //strongSig si //SZ: need to state the precise agile INT-CMA assumption, with a designated hash algorithm and a set of hash algorithms allowed in signing queries
   //CF * hashAlg for certs?
@@ -372,17 +371,17 @@ let strongHS si =
 // Safety of nego crypto processing
 
 // Safe handshake for PMS-based extraction
-let safeCRE si = honestMS (msid si)
+//let safeCRE si = honestMS (msid si)
 
 // Safe handshake for MS-based VerifyData
-let safeVD si = honestMS (msid si) && strongVD(vdAlg si)
+//let safeVD si = honestMS (msid si) && strongVD(vdAlg si)
 //MK: safeVD is used for idealization even if ciphersuites don't match.
 //MK: this is needed to guarantee security of finished message MACs
 
 assume val int_cma: macAlg -> Tot bool
 let strongAuthSI si = true //TODO: fix
 
-assume val strongAESI: nego -> Tot bool
+assume val strongAESI: sessionInfo -> Tot bool
 
 // -------------------------------------------------------------------
 // Indexing instances of derived keys for AE etc. 
@@ -639,30 +638,26 @@ type id =
 | ID12: pv:protocolVersion{pv <> TLS_1p3} -> msId:msId -> kdfAlg:kdfAlg_t -> aeAlg: aeAlg -> cr:crand -> sr:srand -> writer:role -> id 
 
 (* type nego = { *)
-(*   n_resume: bool; *)
-(*   n_client_random: random; *)
-(*   n_server_random: random; *)
-(*   n_sessionID: option sessionID; *)
-(*   n_protocol_version: protocolVersion; *)
-(*   n_kexAlg: kexAlg; *)
-(*   n_aeAlg: aeAlg; *)
-(*   n_sigAlg: option sigAlg; *)
-(*   n_cipher_suite: cipherSuite; *)
-(*   n_dh_group: option namedGroup; *)
-(*   n_compression: option compression; *)
-(*   n_extensions: negotiatedExtensions; *)
-(*   n_scsv: list scsv_suite; *)
+(*   si_resume: bool; *)
+(*   si_client_random: random; *)
+(*   si_server_random: random; *)
+(*   si_sessionID: option sessionID; *)
+(*   si_protocol_version: protocolVersion; *)
+(*   si_kexAlg: kexAlg; *)
+(*   si_aeAlg: aeAlg; *)
+(*   si_sigAlg: option sigAlg; *)
+(*   si_cipher_suite: cipherSuite; *)
+(*   si_dh_group: option namedGroup; *)
+(*   si_compression: option compression; *)
+(*   si_extensions: negotiatedExtensions; *)
+(*   si_scsv: list scsv_suite; *)
 (* } *)
-
-type session = {
-  session_nego: nego;
-}
 
 // represents the outcome of a successful handshake,
 // providing context for the derived epoch
 type handshake =
-  | FreshSession of session // was nego
-  | ResumedSession of session // was abbrInfo * nego
+  | FreshSession of sessionInfo // was nego
+  | ResumedSession of sessionInfo // was abbrInfo * nego
 // We use SessionInfo as unique session indexes.
 // We tried using instead hs, but this creates circularities
 // We'll probably need a global log to reason about them.
@@ -676,14 +671,16 @@ let peerId = function
   ID13 kid
 | ID12 pv msid kdf ae cr sr rw -> ID12 pv msid kdf ae cr sr (dualRole rw)
 
-val siId: si:nego{ 
-  is_Some (prfMacAlg_of_ciphersuite_aux (si.n_cipher_suite)) /\ 
-  si.n_protocol_version = TLS_1p2 /\
-  pvcs si.n_protocol_version si.n_cipher_suite } -> role -> Tot id
+(*
+val siId: si:sessionInfo{ 
+  is_Some (prfMacAlg_of_ciphersuite_aux (si.si_cipher_suite)) /\ 
+  si.si_protocol_version = TLS_1p2 /\
+  pvcs si.si_protocol_version si.si_cipher_suite } -> role -> Tot id
 
 let siId si r =
   let cr, sr = split (csrands si) 32 in
-  ID12 si.n_protocol_version (msid si) (kdfAlg si.n_protocol_version si.n_cipher_suite) (siAuthEncAlg si) cr sr r
+  ID12 si.si_protocol_version (msid si) (kdfAlg si.si_protocol_version si.si_cipher_suite) (siAuthEncAlg si) cr sr r
+*)
 
 let pv_of_id (i:id{~(is_PlaintextID i)}) = match i with
   | ID13 _ -> TLS_1p3
@@ -726,7 +723,7 @@ let lemma_ID12 (i:id)
   = ()
 
 // Pretty printing
-let sinfo_to_string (si:nego) = "TODO"
+let sinfo_to_string (si:sessionInfo) = "TODO"
 
 // -----------------------------------------------------------------------
 // Safety of key derivation depends on matching algorithms (see PRF)
